Working prototypes.

GroupEqPrototype.v
@@ -1,6 +1,6 @@
-From Coq Require Extraction ZArith.
-
 Set Warnings "-notation-overridden".
+
+From Coq Require Extraction ZArith.
 
 Module Classes.
 
@@ -11,16 +11,7 @@ Class Inv (A : Type) : Type := inv : A -> A.
 Notation "x '+' y" := (opr x y).
 Notation "'0'" := idn.
 Notation "'-' x" := (inv x).
-
-Class Group (A : Type) {opr : Opr A} {idn : Idn A} {inv : Inv A} : Prop := {
-  ass : forall x y z : A, (x + y) + z = x + (y + z);
-  idn_l : forall x : A, 0 + x = x;
-  idn_r : forall x : A, x + 0 = x;
-  inv_l : forall x : A, (- x) + x = 0;
-  inv_r : forall x : A, x + (- x) = 0;
-}.
-
-Module WeakHierarchy.
+Notation "x '-' y" := (x + (- y)).
 
 Class Semigroup (A : Type) {opr : Opr A} : Prop := {
   ass : forall x y z : A, (x + y) + z = x + (y + z);
@@ -38,8 +29,6 @@ Class Group (A : Type) {opr : Opr A} {idn : Idn A} {inv : Inv A} : Prop := {
   inv_r : forall x : A, x + (- x) = 0;
 }.
 
-End WeakHierarchy.
-
 End Classes.
 
 Module Properties.
@@ -51,7 +40,7 @@ Theorem ivl : forall {A : Type}
   forall x : A, - (- x) = x.
 Proof.
   intros A opr idn inv grp x.
-  destruct grp as [pa pnl pnr pvl pvr].
+  destruct grp as [[[pa] pnl pnr] pvl pvr].
   rewrite <- (pnr (- (- x))). rewrite <- (pvl x).
   rewrite <- (pa (- (- x)) (- x) x). rewrite (pvl (- x)). rewrite (pnl x).
   reflexivity. Qed.
@@ -61,7 +50,7 @@ Lemma inj_l : forall {A : Type}
   forall x y z : A, z + x = z + y -> x = y.
 Proof.
   intros A opr idn inv grp x y z p.
-  destruct grp as [pa pnl pnr pvl pvr].
+  destruct grp as [[[pa] pnl pnr] pvl pvr].
   rewrite <- (pnl x). rewrite <- (pvl z). rewrite (pa (- z) z x).
   rewrite p. rewrite <- (pa (- z) z y). rewrite (pvl z). rewrite (pnl y).
   reflexivity. Qed.
@@ -71,7 +60,7 @@ Lemma inj_r : forall {A : Type}
   forall x y z : A, x + z = y + z -> x = y.
 Proof.
   intros A opr idn inv grp x y z p.
-  destruct grp as [pa pnl pnr pvl pvr].
+  destruct grp as [[[pa] pnl pnr] pvl pvr].
   rewrite <- (pnr x). rewrite <- (pvr z). rewrite <- (pa x z (- z)).
   rewrite p. rewrite (pa y z (- z)). rewrite (pvr z). rewrite (pnr y).
   reflexivity. Qed.
@@ -82,7 +71,7 @@ Theorem dis : forall {A : Type}
 Proof.
   intros A opr idn inv grp x y.
   apply (inj_l (- (y + x)) ((- x) + (- y)) (y + x)).
-  destruct grp as [pa pnl pnr pvl pvr].
+  destruct grp as [[[pa] pnl pnr] pvl pvr].
   rewrite (pvr (y + x)). rewrite <- (pa (y + x) (- x) (- y)).
   rewrite (pa y x (- x)). rewrite (pvr x). rewrite (pnr y). rewrite (pvr y).
   reflexivity. Qed.
@@ -96,33 +85,12 @@ Import Classes ZArith Z.
 Open Scope Z_scope.
 
 Instance Z_Opr : Opr Z := fun x y : Z => x + y.
-Instance Z_Idn : Idn Z := 0.
-Instance Z_Inv : Inv Z := fun x => - x.
-
-Instance Z_Group : Group Z := {
-  ass := _;
-  idn_l := _; idn_r := _;
-  inv_l := _; inv_r := _;
-}.
-Proof.
-  all: cbv [Classes.opr Z_Opr Classes.idn Z_Idn Classes.inv Z_Inv].
-  - intros x y z. rewrite add_assoc. reflexivity.
-  - intros x. rewrite add_0_l. reflexivity.
-  - intros x. rewrite add_0_r. reflexivity.
-  - intros x. rewrite add_opp_diag_l. reflexivity.
-  - intros x. rewrite add_opp_diag_r. reflexivity. Qed.
-
-Module WeakestHierarchy.
-
-Import WeakHierarchy.
-
-Instance Z_Opr : Opr Z := fun x y : Z => x + y.
 
 Instance Z_Semigroup : Semigroup Z := {
   ass := _;
 }.
 Proof.
-  all: cbv [Classes.opr Z_Opr Classes.idn Z_Idn Classes.inv Z_Inv].
+  all: cbv [Classes.opr Z_Opr].
   - intros x y z. rewrite add_assoc. reflexivity. Qed.
 
 Instance Z_Idn : Idn Z := 0.
@@ -131,7 +99,7 @@ Instance Z_Monoid : Monoid Z := {
   idn_l := _; idn_r := _;
 }.
 Proof.
-  all: cbv [Classes.opr Z_Opr Classes.idn Z_Idn Classes.inv Z_Inv].
+  all: cbv [Classes.opr Z_Opr Classes.idn Z_Idn].
   - intros x. rewrite add_0_l. reflexivity.
   - intros x. rewrite add_0_r. reflexivity. Qed.
 
@@ -144,8 +112,6 @@ Proof.
   all: cbv [Classes.opr Z_Opr Classes.idn Z_Idn Classes.inv Z_Inv].
   - intros x. rewrite add_opp_diag_l. reflexivity.
   - intros x. rewrite add_opp_diag_r. reflexivity. Qed.
-
-End WeakestHierarchy.
 
 End Instances.
 
@@ -166,7 +132,7 @@ Section Output.
 
 Import Classes.
 
-Example fate := meaning + (- luck).
+Example fate := meaning - luck.
 
 End Output.
 
