RingEqPrototype.v
@@ -1,28 +1,12 @@
-From Coq Require Extraction ZArith.
-
 Set Warnings "-notation-overridden".
+
+From Coq Require Extraction ZArith.
 
 Module Classes.
 
 Class Opr (A : Type) : Type := opr : A -> A -> A.
 Class Idn (A : Type) : Type := idn : A.
 Class Inv (A : Type) : Type := inv : A -> A.
-
-Local Notation "x '+' y" := (opr x y).
-Local Notation "'0'" := idn.
-Local Notation "'-' x" := (inv x).
-Local Notation "x '*' y" := (opr x y).
-Local Notation "'1'" := idn.
-Local Notation "'/' x" := (inv x).
-
-Class Group (A : Type) {opr : Opr A} {idn : Idn A} {inv : Inv A} : Prop := {
-  ass : forall x y z : A, (x + y) + z = x + (y + z);
-  idn_l : forall x : A, 0 + x = x;
-  idn_r : forall x : A, x + 0 = x;
-  inv_l : forall x : A, (- x) + x = 0;
-  inv_r : forall x : A, x + (- x) = 0;
-}.
-
 Class Add (A : Type) : Type := add : A -> A -> A.
 Class Zero (A : Type) : Type := zero : A.
 Class Neg (A : Type) : Type := neg : A -> A.
@@ -33,30 +17,33 @@ Class Recip (A : Type) : Type := recip : A -> A.
 Notation "x '+' y" := (add x y).
 Notation "'0'" := zero.
 Notation "'-' x" := (neg x).
+Notation "x '-' y" := (x + (- y)).
 Notation "x '*' y" := (mul x y).
 Notation "'1'" := one.
 Notation "'/' x" := (recip x).
+Notation "x '/' y" := (x * (/ y)).
 
-Class Ring (A : Type) {add : Add A} {zero : Zero A} {neg : Neg A}
-  {mul : Mul A} {one : One A} : Prop := {
-  add_ass : forall x y z : A, (x + y) + z = x + (y + z);
-  add_idn_l : forall x : A, 0 + x = x;
-  add_idn_r : forall x : A, x + 0 = x;
-  add_inv_l : forall x : A, (- x) + x = 0;
-  add_inv_r : forall x : A, x + (- x) = 0;
-  add_com : forall x y : A, y + x = x + y;
-  mul_ass : forall x y z : A, (x * y) * z = x * (y * z);
-  mul_idn_l : forall x : A, 1 * x = x;
-  mul_idn_r : forall x : A, x * 1 = x;
-  dis_l : forall x y z : A, x * (y + z) = x * y + x * z;
-  dis_r : forall x y z : A, (x + y) * z = x * z + y * z;
-}.
+Module AdditiveNotations.
 
-Module WeakHierarchy.
+Notation "x '+' y" := (opr x y).
+Notation "'0'" := idn.
+Notation "'-' x" := (inv x).
+Notation "x '-' y" := (x + (- y)).
 
-Local Notation "x '+' y" := (opr x y).
-Local Notation "'0'" := idn.
-Local Notation "'-' x" := (inv x).
+End AdditiveNotations.
+
+Module MultiplicativeNotations.
+
+Notation "x '*' y" := (opr x y).
+Notation "'1'" := idn.
+Notation "'/' x" := (inv x).
+Notation "x '/' y" := (x * (/ y)).
+
+End MultiplicativeNotations.
+
+Section Additive.
+
+Import AdditiveNotations.
 
 Class Semigroup (A : Type) {opr : Opr A} : Prop := {
   ass : forall x y z : A, (x + y) + z = x + (y + z);
@@ -74,40 +61,29 @@ Class Group (A : Type) {opr : Opr A} {idn : Idn A} {inv : Inv A} : Prop := {
   inv_r : forall x : A, x + (- x) = 0;
 }.
 
-Notation "x '+' y" := (add x y).
-Notation "'0'" := zero.
-Notation "'-' x" := (neg x).
-Notation "x '*' y" := (mul x y).
-Notation "'1'" := one.
-Notation "'/' x" := (recip x).
+End Additive.
 
 Class Ring (A : Type) {add : Add A} {zero : Zero A} {neg : Neg A}
   {mul : Mul A} {one : One A} : Prop := {
   add_group :> Group A (opr := add) (idn := zero) (inv := neg);
-  add_com : forall x y : A, y + x = x + y;
+  add_com : forall x y : A, x + y = y + x;
   mul_monoid :> Monoid A (opr := mul) (idn := one);
   dis_l : forall x y z : A, x * (y + z) = x * y + x * z;
   dis_r : forall x y z : A, (x + y) * z = x * z + y * z;
 }.
 
-End WeakHierarchy.
-
 End Classes.
 
 Module Properties.
 
-Import Classes.
-
-Local Notation "x '+' y" := (opr x y).
-Local Notation "'0'" := idn.
-Local Notation "'-' x" := (inv x).
+Import Classes AdditiveNotations.
 
 Theorem ivl : forall {A : Type}
   {opr : Opr A} {idn : Idn A} {inv : Inv A} {grp : Group A},
   forall x : A, - (- x) = x.
 Proof.
   intros A opr idn inv grp x.
-  destruct grp as [pa pnl pnr pvl pvr].
+  destruct grp as [[[pa] pnl pnr] pvl pvr].
   rewrite <- (pnr (- (- x))). rewrite <- (pvl x).
   rewrite <- (pa (- (- x)) (- x) x). rewrite (pvl (- x)). rewrite (pnl x).
   reflexivity. Qed.
@@ -117,7 +93,7 @@ Lemma inj_l : forall {A : Type}
   forall x y z : A, z + x = z + y -> x = y.
 Proof.
   intros A opr idn inv grp x y z p.
-  destruct grp as [pa pnl pnr pvl pvr].
+  destruct grp as [[[pa] pnl pnr] pvl pvr].
   rewrite <- (pnl x). rewrite <- (pvl z). rewrite (pa (- z) z x).
   rewrite p. rewrite <- (pa (- z) z y). rewrite (pvl z). rewrite (pnl y).
   reflexivity. Qed.
@@ -127,7 +103,7 @@ Lemma inj_r : forall {A : Type}
   forall x y z : A, x + z = y + z -> x = y.
 Proof.
   intros A opr idn inv grp x y z p.
-  destruct grp as [pa pnl pnr pvl pvr].
+  destruct grp as [[[pa] pnl pnr] pvl pvr].
   rewrite <- (pnr x). rewrite <- (pvr z). rewrite <- (pa x z (- z)).
   rewrite p. rewrite (pa y z (- z)). rewrite (pvr z). rewrite (pnr y).
   reflexivity. Qed.
@@ -138,7 +114,7 @@ Theorem dis : forall {A : Type}
 Proof.
   intros A opr idn inv grp x y.
   apply (inj_l (- (y + x)) ((- x) + (- y)) (y + x)).
-  destruct grp as [pa pnl pnr pvl pvr].
+  destruct grp as [[[pa] pnl pnr] pvl pvr].
   rewrite (pvr (y + x)). rewrite <- (pa (y + x) (- x) (- y)).
   rewrite (pa y x (- x)). rewrite (pvr x). rewrite (pnr y). rewrite (pvr y).
   reflexivity. Qed.
@@ -151,63 +127,13 @@ Import Classes ZArith Z.
 
 Open Scope Z_scope.
 
-Instance Z_Opr : Opr Z := fun x y : Z => x + y.
-Instance Z_Idn : Idn Z := 0.
-Instance Z_Inv : Inv Z := fun x => - x.
-
-Instance Z_Group : Group Z := {
-  ass := _;
-  idn_l := _; idn_r := _;
-  inv_l := _; inv_r := _;
-}.
-Proof.
-  all: cbv [Classes.opr Z_Opr Classes.idn Z_Idn Classes.inv Z_Inv].
-  - intros x y z. rewrite add_assoc. reflexivity.
-  - intros x. rewrite add_0_l. reflexivity.
-  - intros x. rewrite add_0_r. reflexivity.
-  - intros x. rewrite add_opp_diag_l. reflexivity.
-  - intros x. rewrite add_opp_diag_r. reflexivity. Qed.
-
-Instance Z_Add : Add Z := fun x y : Z => x + y.
-Instance Z_Zero : Zero Z := 0.
-Instance Z_Neg : Neg Z := fun x => - x.
-Instance Z_Mul : Mul Z := fun x y : Z => x * y.
-Instance Z_One : One Z := 1.
-
-Instance Z_Ring : Ring Z := {
-  add_ass := _;
-  add_idn_l := _; add_idn_r := _;
-  add_inv_l := _; add_inv_r := _;
-  add_com := _;
-  mul_ass := _;
-  mul_idn_l := _; mul_idn_r := _;
-  dis_l := _; dis_r := _;
-}.
-Proof.
-  all: cbv [Classes.add Z_Add Classes.neg Z_Neg Classes.mul Z_Mul].
-  - intros x y z. rewrite add_assoc. reflexivity.
-  - intros x. rewrite add_0_l. reflexivity.
-  - intros x. rewrite add_0_r. reflexivity.
-  - intros x. rewrite add_opp_diag_l. reflexivity.
-  - intros x. rewrite add_opp_diag_r. reflexivity.
-  - intros x y. rewrite add_comm. reflexivity.
-  - intros x y z. rewrite mul_assoc. reflexivity.
-  - intros x. rewrite mul_1_l. reflexivity.
-  - intros x. rewrite mul_1_r. reflexivity.
-  - intros x y z. rewrite mul_add_distr_l. reflexivity.
-  - intros x y z. rewrite mul_add_distr_r. reflexivity. Qed.
-
-Module WeakestHierarchy.
-
-Import WeakHierarchy.
-
 Instance Z_AddOpr : Opr Z := fun x y : Z => x + y.
 
 Instance Z_AddSemigroup : Semigroup Z := {
   ass := _;
 }.
 Proof.
-  all: cbv [Classes.opr Z_Opr Classes.idn Z_Idn Classes.inv Z_Inv].
+  all: cbv [Classes.opr Z_AddOpr].
   - intros x y z. rewrite add_assoc. reflexivity. Qed.
 
 Instance Z_AddIdn : Idn Z := 0.
@@ -216,7 +142,7 @@ Instance Z_AddMonoid : Monoid Z := {
   idn_l := _; idn_r := _;
 }.
 Proof.
-  all: cbv [Classes.opr Z_Opr Classes.idn Z_Idn Classes.inv Z_Inv].
+  all: cbv [Classes.opr Z_AddOpr Classes.idn Z_AddIdn].
   - intros x. rewrite add_0_l. reflexivity.
   - intros x. rewrite add_0_r. reflexivity. Qed.
 
@@ -226,7 +152,7 @@ Instance Z_AddGroup : Group Z := {
   inv_l := _; inv_r := _;
 }.
 Proof.
-  all: cbv [Classes.opr Z_Opr Classes.idn Z_Idn Classes.inv Z_Inv].
+  all: cbv [Classes.opr Z_AddOpr Classes.idn Z_AddIdn Classes.inv Z_AddInv].
   - intros x. rewrite add_opp_diag_l. reflexivity.
   - intros x. rewrite add_opp_diag_r. reflexivity. Qed.
 
@@ -236,7 +162,7 @@ Instance Z_MulSemigroup : Semigroup Z := {
   ass := _;
 }.
 Proof.
-  all: cbv [Classes.opr Z_Opr Classes.idn Z_Idn Classes.inv Z_Inv].
+  all: cbv [Classes.opr Z_MulOpr].
   - intros x y z. rewrite mul_assoc. reflexivity. Qed.
 
 Instance Z_MulIdn : Idn Z := 1.
@@ -245,7 +171,7 @@ Instance Z_MulMonoid : Monoid Z := {
   idn_l := _; idn_r := _;
 }.
 Proof.
-  all: cbv [Classes.opr Z_Opr Classes.idn Z_Idn Classes.inv Z_Inv].
+  all: cbv [Classes.opr Z_MulOpr Classes.idn Z_MulIdn].
   - intros x. rewrite mul_1_l. reflexivity.
   - intros x. rewrite mul_1_r. reflexivity. Qed.
 
@@ -260,12 +186,12 @@ Instance Z_Ring : Ring Z := {
   dis_l := _; dis_r := _;
 }.
 Proof.
-  all: cbv [Classes.add Z_Add Classes.neg Z_Neg Classes.mul Z_Mul].
-  - intros x y. rewrite Z.add_comm. reflexivity.
+  all: cbv [Classes.add Z_Add Classes.zero Z_Zero Classes.neg Z_Neg
+    Classes.mul Z_Mul Classes.one Z_One].
+  all: cbv [Z_AddOpr Z_AddIdn Z_AddInv Z_MulOpr Z_MulIdn].
+  - intros x y. rewrite add_comm. reflexivity.
   - intros x y z. rewrite mul_add_distr_l. reflexivity.
   - intros x y z. rewrite mul_add_distr_r. reflexivity. Qed.
-
-End WeakestHierarchy.
 
 End Instances.
 
